Temporal transition proofs in progress

theories/Environments_Contexts/REnvironment.v
@@ -14,9 +14,8 @@ Include Ext.
 Import Raw OP.P.
 
 (** *** Definition *)
-(*
-Definition embeds_func V v := 
-    add (new_key V) ([⧐ᵣₓ (new_key V) ≤ 1 ] ⩽ v … ⩾) (shift (new_key V) 1 V).
+
+Definition embeds_func V v := add (new_key V) (⩽ v … ⩾) V.
 
 Definition embeds_func_revert v V := embeds_func V v. 
 
@@ -34,7 +33,6 @@ Definition extracts (V : REnvironment.t) : list (option Λ) :=
                         | Some _ => None
                         | None   => None
                       end) (seq 0 (max_key V)).
-*)
 
 Definition halts (V : REnvironment.t) := forall (r : resource) (v : 𝑣), 
  find r V = Some v -> halts (Cell.extract v).
@@ -43,14 +41,12 @@ Definition used r (V : REnvironment.t) := exists v, find r V = Some (⩽ … v �
 Definition unused r (V : REnvironment.t) := exists v, find r V = Some (⩽ v … ⩾).
 
 (** *** Embedding *)
-(*
+
 Lemma embedding_func_new_spec : forall V v,
  new_key (embeds_func_revert v V) = S (new_key V).
 Proof.
   unfold embeds_func_revert, embeds_func; intros.
-  rewrite new_key_add_spec_1; auto.
-  - apply shift_new_notin_spec; lia.
-  - rewrite shift_new_spec; lia.
+  rewrite new_key_add_spec_1; auto; apply new_key_notin_spec; lia.
 Qed.
 
 Lemma embedding_func_in_spec : forall V v r,
@@ -58,14 +54,7 @@ Lemma embedding_func_in_spec : forall V v r,
 Proof. 
   split; intros; unfold embeds_func_revert,embeds_func in *.
   - rewrite add_in_iff in H; destruct H; auto.
-    right. apply new_key_in_spec in H as H'.
-    rewrite shift_new_spec in H'; auto.
-    rewrite shift_in_spec with (lb := (new_key V)) (k := 1).
-    rewrite Resource.shift_valid_refl; auto.
   - destruct H; rewrite add_in_iff; subst; auto.
-    right. apply new_key_in_spec in H as H'.
-    rewrite shift_in_spec with (lb := (new_key V)) (k := 1) in H.
-    rewrite Resource.shift_valid_refl in H; auto.
 Qed.
 
 Lemma embedding_func_unused_spec : forall r x V,
@@ -73,11 +62,8 @@ Lemma embedding_func_unused_spec : forall r x V,
 Proof.
   intros; unfold embeds_func_revert,embeds_func.
   destruct (Resource.eq_dec r (new_key V)); subst.
-  - simpl. exists <[[⧐ₜₘ {new_key V} ≤ 1] x]>; rewrite add_eq_o; auto.
-  - destruct H. exists <[[⧐ₜₘ {new_key V} ≤ 1] x0]>. rewrite add_neq_o; auto.
-    assert (In r V). { exists (⩽ x0 … ⩾). now apply find_2. }
-    apply new_key_in_spec in H0. rewrite shift_find_spec in H;
-    rewrite Resource.shift_valid_refl in H; eauto.
+  - simpl. exists x; rewrite add_eq_o; auto.
+  - destruct H; exists x0. rewrite add_neq_o; auto.
 Qed.
 
 Lemma embedding_gen_new_spec : forall l V,
@@ -90,22 +76,8 @@ Proof.
   rewrite embedding_func_new_spec; rewrite <- IHl; lia.
 Qed.
 
-Lemma valid_embedding_gen_keys_spec : forall l V,
-  forall r, In r (embeds_gen V l) -> (new_key (embeds_gen V l)) ⊩ᵣ r.
-Proof.
-  intros; unfold embeds_gen in *; rewrite <- fold_left_rev_right in *.
-  fold embeds_func_revert in *. revert V r H.
-  induction l using rev_ind; intros; simpl in *.
-  - now apply new_key_in_spec.
-  - rewrite rev_unit in *; simpl in *; rewrite embedding_func_new_spec.
-    rewrite embedding_func_in_spec in H; destruct H; subst.
-    -- unfold Resource.valid; lia.
-    -- apply IHl in H. apply Resource.valid_weakening 
-       with (k := new_key (fold_right embeds_func_revert V (List.rev l))); auto.
-Qed.
-
 Lemma embedding_gen_find_eq_spec : forall V x,
-  find (new_key V) (embeds_func_revert x V) = Some (⩽ [⧐ₜₘ {new_key V} ≤ 1] x … ⩾).
+  find (new_key V) (embeds_func_revert x V) = Some (⩽ x … ⩾).
 Proof.
   unfold embeds_func_revert, embeds_func; intros.
   rewrite add_eq_o; auto.
@@ -120,8 +92,7 @@ Proof.
   induction l using rev_ind; intros V r H HIn; simpl in *; auto.
   rewrite rev_unit in *; simpl in *.
   rewrite embedding_func_in_spec in HIn. destruct HIn; subst.
-  - exists (Term.shift (new_key (fold_right embeds_func_revert V (List.rev l))) 1 x).
-    apply embedding_gen_find_eq_spec.
+  - exists x. apply embedding_gen_find_eq_spec.
   - apply IHl in H0 as H0'; auto. now apply embedding_func_unused_spec.
 Qed.
 
@@ -131,6 +102,7 @@ Proof.
   intros; unfold embeds in *; apply embedding_gen_unused; auto.
   intros; inversion H0; inversion H1.
 Qed.
+
 
 Lemma embedding_Forall_unused : forall l V,
   For_all (fun _ v => Cell.unused v) V ->
@@ -145,7 +117,7 @@ Proof.
     -- now exists λ.
     -- contradiction.
 Qed. 
-*)
+
 
 (** *** Halts *)
 
